testdata/modules/qualified_import/cue.mod/module.cue
@@ -1,0 +1,4 @@
+module: "qualified.example"
+language: {
+	version: "v0.15.4"
+}
