testdata/modules/qualified_import/lib/math-utils/math.cue
@@ -1,0 +1,5 @@
+package math
+
+Sin:   42
+Pi:    3
+twice: Sin + Sin
