testdata/modules/qualified_import_bare/defs/defs.cue
@@ -1,0 +1,3 @@
+package defs
+
+Answer: 7
