testdata/modules/qualified_import_mixed/lib/math-utils/math.cue
@@ -1,0 +1,3 @@
+package math
+
+Answer: 42
