testdata/modules/qualified_import_mixed/main.cue
@@ -1,0 +1,9 @@
+package main
+
+import (
+	"mixed.example/lib/math-utils:math"
+	"mixed.example/strs"
+)
+
+answer:   math.Answer
+greeting: strs.Greeting
